program_logic/WhileNoSuccess.ec
@@ -56,103 +56,113 @@ module DW = {
 
 
 
+op MyPred : rrt -> bool.
 
 declare module A <: HasRun {-W, -DW}.
 
 declare axiom A_ll : islossless A.run.
 
-declare axiom A_rew_ph x : phoare[ A.run : (glob A) = x ==> (glob A) = x ] = 1%r.
+declare axiom A_rew_ph x : phoare[ A.run : (glob A) = x ==> !MyPred res => (glob A) = x ] = 1%r.
 
-lemma A_rew_h x : hoare[ A.run : (glob A) = x ==> (glob A) = x ] .
+
+
+lemma A_rew_h x : hoare[ A.run : (glob A) = x ==> !MyPred res => (glob A) = x ] .
 bypr. progress. 
 have <- : Pr[A.run(z{m}) @ &m : false ] = 0%r. smt.
-have : 1%r = Pr[A.run(z{m}) @ &m : (glob A) <> (glob A){m} ]
-  + Pr[A.run(z{m}) @ &m : (glob A) = (glob A){m} ].
+have : 1%r = Pr[A.run(z{m}) @ &m : !(!MyPred res => (glob A) = (glob A){m}) ]
+  + Pr[A.run(z{m}) @ &m : !MyPred res => (glob A) = (glob A){m} ].
    have <- :  Pr[A.run(z{m}) @ &m : true ] = 1%r. byphoare. apply  A_ll. auto. auto.
-rewrite Pr[mu_split (glob A) = (glob A){m} ]. smt.
-have ->: Pr[A.run(z{m}) @ &m : (glob A) = (glob A){m} ] = 1%r. byphoare (_: (glob A) = (glob A){m} ==> _). apply (A_rew_ph). auto. auto.
+rewrite Pr[mu_split (!MyPred res => (glob A) = (glob A){m}) ]. smt.
+have ->: Pr[A.run(z{m}) @ &m : (!MyPred res => (glob A) = (glob A){m}) ] = 1%r. byphoare (_: (glob A) = (glob A){m} ==> _). apply (A_rew_ph). auto. auto.
 smt.
 qed.
-  
-lemma asdistr_rew : forall (D : (glob A) -> irt -> rrt distr),
+
+
+
+
+lemma asdistr_rew2 : forall (D : (glob A) -> irt -> rrt distr) ,
   (forall &m M a, mu (D (glob A){m} a) M = Pr[ A.run(a) @ &m :  M res ])
   => forall &m a, equiv [SF.sampleFrom ~ A.run : ={glob A} /\ arg{1} = (D (glob A){m} a) 
                          /\ (glob A){2} = (glob A){m} /\ arg{2} = a 
-                         ==>  res{1} =  res{2} /\ (glob A){2} = (glob A){m} ].
+                         ==>  res{1} =  res{2} /\ (!MyPred res{2}  =>(glob A){2} = (glob A){m}) ].
 progress.
-bypr (res{1}, true) (res{2}, (glob A){2} = (glob A){m}). progress. smt.
+bypr (res{1}, true) (res{2}, !MyPred res{2} => (glob A){2} = (glob A){m}). progress.  smt.
 progress. 
+
 have ->: Pr[SF.sampleFrom(d{1}) @ &1 : (res, true) = a0]
  = Pr[SF.sampleFrom(d{1}) @ &1 : res = a0.`1 /\ a0.`2 = true].
 rewrite Pr[mu_eq]. smt. auto.
-have ->: Pr[A.run(z{2}) @ &2 : (res, (glob A) = (glob A){m}) = a0]
- = Pr[A.run(z{2}) @ &2 : res  = a0.`1 /\ ((glob A) = (glob A){m})  = a0.`2].
+have ->: Pr[A.run(z{2}) @ &2 : (res, (!MyPred res => (glob A) = (glob A){m})) = a0]
+ = Pr[A.run(z{2}) @ &2 : res  = a0.`1 /\ (!MyPred res => (glob A) = (glob A){m})  = a0.`2].
 rewrite Pr[mu_eq]. smt. auto.
-case (a0.`2 = true). 
+case (a0.`2 = true).
 progress. rewrite H3. simplify.
 have -> : Pr[A.run(z{2}) @ &2 :
-   res = a0.`1 /\ ((glob A) = (glob A){m}) = true]
+   res = a0.`1 /\ (!MyPred res => (glob A) = (glob A){m}) = true]
  = Pr[A.run(z{2}) @ &2 :
-   res = a0.`1]. 
+   res = a0.`1].
 
-  have kj: Pr[A.run(z{2}) @ &2 : res = a0.`1 /\ ((glob A) = (glob A){m}) = false] = 0%r.
-   have : Pr[A.run(z{2}) @ &2 : ((glob A) <> (glob A){m})] = 0%r.      
+  have kj: Pr[A.run(z{2}) @ &2 : res = a0.`1 /\ (!MyPred res => (glob A) = (glob A){m}) = false] = 0%r.
+   have : Pr[A.run(z{2}) @ &2 : !(!MyPred res => (glob A) = (glob A){m})] = 0%r.
    rewrite - H2.
    byphoare (_: (glob A) = (glob A){2} ==> _ ). hoare.  simplify.
-    have f : forall ga, phoare[ A.run : (glob A) = ga ==> (glob A) = ga] = 1%r. 
+    have f : forall ga, phoare[ A.run : (glob A) = ga ==>  (!MyPred res => (glob A) = ga) ] = 1%r.
     move => ga. apply A_rew_ph.  apply A_rew_h. auto. auto.
      smt.
-smt.  
-byequiv (_: ={glob A} /\ arg{2} = z{2} /\ (glob A){2} = (glob A){m} /\ arg{1} = D (glob A){m} z{2} ==> _). 
+smt.
+byequiv (_: ={glob A} /\ arg{2} = z{2} /\ (glob A){2} = (glob A){m} /\ arg{1} = D (glob A){m} z{2} ==> _).
 exists* z{2}. elim*. progress.
 proc*.
 call  (asdistr A D H &m arg_R ).
-auto. progress. auto. 
+auto. progress. auto.
 move => hp.
 have hpp : a0.`2 = false. smt.
 clear hp.
 rewrite hpp.
   have ->: Pr[SF.sampleFrom(d{1}) @ &1 : res = a0.`1 /\ false] = 0%r.
   smt.
-  have ->: Pr[A.run(z{2}) @ &2 : res = a0.`1 /\ ((glob A) = (glob A){m}) = false] = 0%r.
-   have : Pr[A.run(z{2}) @ &2 : ((glob A) <> (glob A){m})] = 0%r.      
+  have ->: Pr[A.run(z{2}) @ &2 : res = a0.`1 /\ (!MyPred res => (glob A) = (glob A){m}) = false] = 0%r.
+   have : Pr[A.run(z{2}) @ &2 : !(!MyPred res => (glob A) = (glob A){m}) ] = 0%r.
    rewrite - H2.
    byphoare (_: (glob A) = (glob A){2} ==> _ ). hoare.  simplify.
-    have f : forall ga, phoare[ A.run : (glob A) = ga ==> (glob A) = ga] = 1%r. 
+    have f : forall ga, phoare[ A.run : (glob A) = ga ==> (!MyPred res => (glob A) = ga) ] = 1%r.
     move => ga. apply A_rew_ph. apply A_rew_h.  auto. auto.
      smt.
 auto.
 qed.
 
 
+
+
   
-lemma zz MyPa  (da : (glob A) -> irt -> rrt distr) :  
+lemma zz  (da : (glob A) -> irt -> rrt distr) :  
  (forall &m (M : rrt -> bool) (a : irt),
        mu (da (glob A){m} a) M = Pr[A.run(a) @ &m : M res])
- => forall &m P e (s : int) r ia,  
-  Pr[ DW.whp_d(MyPa,da (glob A){m} ia,s,e,r) @ &m : P res ]
-   = Pr[ W(A).whp(MyPa,ia, s,e,r) @ &m : P res ].
+ => forall &m P e (s : int) rr ia,  
+  Pr[ DW.whp_d(MyPred,da (glob A){m} ia,s,e,rr) @ &m : P res ]
+   = Pr[ W(A).whp(MyPred,ia, s,e,rr) @ &m : P res ].
 progress. 
-byequiv (_: ={p,s,e,r, glob A} /\ d{1} = (da (glob A){m} ia) /\ i{2} = ia
+byequiv (_: ={p,s,e,r, glob A} /\ d{1} = (da (glob A){m} ia) /\ i{2} = ia /\ p{1} = MyPred
      /\ (glob A){2} = (glob A){m} ==> _). proc.
 sp. 
 exists* (glob A){2} . elim*. progress.
-while (={p,r,e,glob A} /\ DW.c{1} = W.c{2} /\ d{1} = da (glob A){m} ia /\ i{2} = ia /\ (glob A){m} = (glob A){2}).
+while (={p,r,e} /\ DW.c{1} = W.c{2} /\ d{1} = da (glob A){m} ia /\ i{2} = ia /\   p{1} = MyPred /\ (!p{1} r{2} => ={glob A} /\ (glob A){2} = (glob A){m}) ).
 wp.
-call (asdistr_rew  da H &m ia).
-skip. progress.    progress.
-progress. auto.
+
+call (asdistr_rew2  da H &m ia).
+skip. progress.    smt.  smt.  smt. smt. skip. progress. smt.
+progress. 
 qed.
 
 
 
-lemma final_zz &m (p : real) MyPa i e ra :  MyPa ra = false => 0 <= e =>
-   Pr[ A.run(i) @ &m : !MyPa res ]  = p
-  => Pr[ W(A).whp(MyPa,i, 1,e,ra) @ &m : !MyPa res ] = (p ^ (e)).
+lemma final_zz &m (p : real)  i e ra :  MyPred ra = false => 0 <= e =>
+   Pr[ A.run(i) @ &m : !MyPred res ]  = p
+  => Pr[ W(A).whp(MyPred,i, 1,e,ra) @ &m : !MyPred res ] = (p ^ (e)).
 case (e = 0).
 progress.
-have ->: Pr[A.run(i) @ &m : ! MyPa res] ^ 0 = 1%r. smt.
-byphoare (_: e = 0 /\ s = 1 /\ MyPa ra = false /\ r = ra ==> _).
+have ->: Pr[A.run(i) @ &m : ! MyPred res] ^ 0 = 1%r. smt.
+byphoare (_: e = 0 /\ s = 1 /\ MyPred ra = false /\ r = ra ==> _).
 simplify. proc. 
 sp.
 rcondf 1. skip. progress. skip. smt. smt. auto.  auto. 
@@ -164,29 +174,29 @@ have exD :  exists (D : (glob A) -> irt -> rrt distr),
         mu (D (glob A){m} a) M = Pr[A.run(a) @ &m : M res].
 apply (reflection_simple_res A).
 elim exD. progress. 
-rewrite - (zz MyPa D H0 &m (fun x => !MyPa x)).
-have ->: Pr[DW.whp_d(MyPa, D (glob A){m} i, 1, e' + 1 , ra) @ &m : !MyPa res]
- = Pr[M.whp(MyPa, D (glob A){m} i, 1, e' + 1 , ra) @ &m : !MyPa res].
+rewrite - (zz  D H0 &m (fun x => !MyPred x)).
+have ->: Pr[DW.whp_d(MyPred, D (glob A){m} i, 1, e' + 1 , ra) @ &m : !MyPred res]
+ = Pr[M.whp(MyPred, D (glob A){m} i, 1, e' + 1 , ra) @ &m : !MyPred res].
 byequiv. proc. simplify.  sp. 
 conseq (_: ={e,r} /\ p{1} = MyP{2} /\ DW.c{1} = M.c{2} /\ d{1} = myd{2}  ==> _). auto.
 while (={e,r} /\ p{1} = MyP{2} /\ DW.c{1} = M.c{2} /\ d{1} = myd{2}). wp. inline*. wp.  rnd. wp. 
 skip. progress. 
 skip. progress. auto. auto.
-byphoare(_: arg = (MyPa,D (glob A){m} i, 1, e' + 1 , ra ) ==> _).
+byphoare(_: arg = (MyPred,D (glob A){m} i, 1, e' + 1 , ra ) ==> _).
 
-have lf :   mu (D (glob A){m} i) (fun (x : rrt) => ! MyPa x) =
-  Pr[A.run(i) @ &m : ! MyPa res].
+have lf :   mu (D (glob A){m} i) (fun (x : rrt) => ! MyPred x) =
+  Pr[A.run(i) @ &m : ! MyPred res].
 rewrite H0. auto.
 
-conseq (asdsadq (Pr[A.run(i) @ &m : ! MyPa res]) MyPa  ra (D (glob A){m} i) lf sf e' H ). auto.
+conseq (asdsadq (Pr[A.run(i) @ &m : ! MyPred res]) MyPred  ra (D (glob A){m} i) lf sf e' H ). auto.
 auto.
 qed.
 
 
 
-lemma final_zz_le &m pr MyPa i e ra :  MyPa ra = false => 0 <= e =>
-   Pr[ A.run(i) @ &m : !MyPa res ]  <= pr
-  => Pr[ W(A).whp(MyPa,i, 1,e,ra) @ &m : !MyPa res ] <= (pr ^ (e)).
+lemma final_zz_le &m pr  i e ra :  MyPred ra = false => 0 <= e =>
+   Pr[ A.run(i) @ &m : !MyPred res ]  <= pr
+  => Pr[ W(A).whp(MyPred,i, 1,e,ra) @ &m : !MyPred res ] <= (pr ^ (e)).
 case (e = 0).
 progress.
 byphoare (_: e = 0 /\ s = 1 /\ p ra = false /\ r = ra ==> _).
@@ -201,33 +211,33 @@ have exD :  exists (D : (glob A) -> irt -> rrt distr),
         mu (D (glob A){m} a) M = Pr[A.run(a) @ &m : M res].
 apply (reflection_simple_res A).
 elim exD. progress. 
-rewrite - (zz MyPa D H1 &m (fun x => !MyPa x)).
-have ->: Pr[DW.whp_d(MyPa,D (glob A){m} i, 1, e' + 1 , ra) @ &m : !MyPa res]
- = Pr[M.whp(MyPa,D (glob A){m} i, 1, e' + 1 , ra) @ &m : !MyPa res].
+rewrite - (zz  D H1 &m (fun x => !MyPred x)).
+have ->: Pr[DW.whp_d(MyPred,D (glob A){m} i, 1, e' + 1 , ra) @ &m : !MyPred res]
+ = Pr[M.whp(MyPred,D (glob A){m} i, 1, e' + 1 , ra) @ &m : !MyPred res].
 byequiv. proc.  sp. 
 conseq (_: ={e,r} /\ p{1} = MyP{2} /\ DW.c{1} = M.c{2} /\ d{1} = myd{2}  ==> _). auto.
 while (={e,r} /\ p{1} = MyP{2} /\ DW.c{1} = M.c{2} /\ d{1} = myd{2}). wp. inline*. wp.  rnd. wp. 
 skip. progress. 
 skip. progress. auto. auto.
-byphoare(_: arg = (MyPa,D (glob A){m} i, 1, e' + 1 , ra ) ==> _).
+byphoare(_: arg = (MyPred,D (glob A){m} i, 1, e' + 1 , ra ) ==> _).
 
-have lf :   mu (D (glob A){m} i) (fun (x : rrt) => ! MyPa x) <= pr. rewrite H1. auto.
-conseq (asdsadq_le pr MyPa ra (D (glob A){m} i) lf sf e' H ). auto.
+have lf :   mu (D (glob A){m} i) (fun (x : rrt) => ! MyPred x) <= pr. rewrite H1. auto.
+conseq (asdsadq_le pr MyPred ra (D (glob A){m} i) lf sf e' H ). auto.
 auto.
 qed.
 
 
 
 
-lemma final_zz_ph_le p MyPa i e r :  MyPa r = false => 0 <= e =>
-   phoare[ A.run : arg = i ==> !MyPa res ] <= p =>
-   phoare [ W(A).whp : arg = (MyPa, i, 1,e,r) ==> !MyPa res ] <= (p ^ (e)).
+lemma final_zz_ph_le p  i e r :  MyPred r = false => 0 <= e =>
+   phoare[ A.run : arg = i ==> !MyPred res ] <= p =>
+   phoare [ W(A).whp : arg = (MyPred, i, 1,e,r) ==> !MyPred res ] <= (p ^ (e)).
 move => sf ep ph1.
 bypr. progress.
-have ff : Pr[A.run(i) @ &m : ! MyPa res] <= p. 
+have ff : Pr[A.run(i) @ &m : ! MyPred res] <= p. 
 byphoare (_: arg = i ==> _). apply ph1. auto. auto.
 rewrite H. simplify.
-apply (final_zz_le &m p MyPa i e r sf ep ff).
+apply (final_zz_le &m p  i e r sf ep ff).
 qed.
 
 
@@ -244,24 +254,24 @@ qed.
 (* qed. *)
 
 
-lemma final_zz_ph &m p MyPa i e r :  MyPa r = false => 0 <= e =>
-   phoare[ A.run : arg = i ==> !MyPa res ] = p =>
-   phoare [ W(A).whp : arg = (MyPa,i, 1,e,r) ==> !MyPa res ] = (p ^ (e)).
+lemma final_zz_ph &m p i e r :  MyPred r = false => 0 <= e =>
+   phoare[ A.run : arg = i ==> !MyPred res ] = p =>
+   phoare [ W(A).whp : arg = (MyPred,i, 1,e,r) ==> !MyPred res ] = (p ^ (e)).
 move => sf ep ph1.
 bypr. progress.
-rewrite -  (final_zz &m0 p MyPa i e r sf ep).
+rewrite -  (final_zz &m0 p  i e r sf ep).
 byphoare (_: arg = i ==> _). conseq ph1. auto. auto.
 rewrite H. auto.
 qed.
 
 
 
-lemma final_zz_ph_m &m p MyPa i e r :  MyPa r = false => 0 <= e =>
-   phoare[ A.run : arg = i /\ (glob A){m} = (glob A) ==> !MyPa res ] = p =>
-   phoare [ W(A).whp : arg = (MyPa,i, 1,e,r) /\ (glob A){m} = (glob A) ==> !MyPa res ] = (p ^ e).
+lemma final_zz_ph_m &m p i e r :  MyPred r = false => 0 <= e =>
+   phoare[ A.run : arg = i /\ (glob A){m} = (glob A) ==> !MyPred res ] = p =>
+   phoare [ W(A).whp : arg = (MyPred,i, 1,e,r) /\ (glob A){m} = (glob A) ==> !MyPred res ] = (p ^ e).
 move => sf ep ph1.
 bypr. progress. rewrite H. simplify.
-rewrite -  (final_zz &m0 p MyPa i e r sf ep). 
+rewrite -  (final_zz &m0 p  i e r sf ep). 
 byphoare (_: arg = i /\ (glob A) = (glob A){m0} ==> _). conseq ph1. auto. auto.
 auto. auto.
 qed.
